Move tsl_param files again (was undo by the PR #14)

translations/tsl_param3.v
@@ -1,305 +1,297 @@
+(* -*- coq-prog-args: ("-type-in-type" "-top" "Translations.tsl_param") -*-  *)
 Require Import Template.All.
-Require Import Arith.Compare_dec.
-From Translations Require Import translation_utils.
-Import String List Lists.List.ListNotations MonadNotation.
-Open Scope list_scope.
-Open Scope string_scope.
+From Translations Require Import translation_utils sigma.
+Import String Lists.List.ListNotations MonadNotation.
+Open Scope list_scope. Open Scope string_scope. Open Scope sigma_scope.
 
-Infix "<=" := Nat.leb.
 
-Definition default_term := tVar "constant_not_found".
-Definition debug_term msg:= tVar ("debug: " ++ msg).
+Reserved Notation "'tsl_ty_param'".
 
-Fixpoint tsl_rec0 (n : nat) (t : term) {struct t} : term :=
+Fixpoint refresh_universes (t : term) {struct t} :=
   match t with
-  | tRel k => if n <= k then tRel (2*k-n+1) else t
-  | tEvar k ts => tEvar k (map (tsl_rec0 n) ts)
-  | tCast t c a => tCast (tsl_rec0 n t) c (tsl_rec0 n a)
-  | tProd na A B => tProd na (tsl_rec0 n A) (tsl_rec0 (n+1) B)
-  | tLambda na A t => tLambda na (tsl_rec0 n A) (tsl_rec0 (n+1) t)
-  | tLetIn na t A u => tLetIn na (tsl_rec0 n t) (tsl_rec0 n A) (tsl_rec0 (n+1) u)
-  | tApp t lu => tApp (tsl_rec0 n t) (map (tsl_rec0 n) lu)
-  | tCase ik t u br => tCase ik (tsl_rec0 n t) (tsl_rec0 n u)
-                            (map (fun x => (fst x, tsl_rec0 n (snd x))) br)
-  | tProj p t => tProj p (tsl_rec0 n t)
-  (* | tFix : mfixpoint term -> nat -> term *)
-  (* | tCoFix : mfixpoint term -> nat -> term *)
+  | tSort s => tSort []
+  | tProd na b t => tProd na b (refresh_universes t)
+  | tLetIn na b t' t => tLetIn na b t' (refresh_universes t)
   | _ => t
   end.
 
-Fixpoint tsl_rec1_app (app : option term) (E : tsl_table) (t : term) : term :=
-  let tsl_rec1 := tsl_rec1_app None in
-  let debug case symbol :=
-      debug_term ("tsl_rec1: " ++ case ++ " " ++ symbol ++ " not found") in
+(* if b it is the first translation, else the second *)
+Fixpoint tsl_rec (fuel : nat) (Σ : global_context) (E : tsl_table) (Γ : context) (b : bool) (t : term) {struct fuel}
+  : tsl_result term :=
+  match fuel with
+  | O => raise NotEnoughFuel
+  | S fuel =>
   match t with
-  | tLambda na A t =>
-    let A0 := tsl_rec0 0 A in
-    let A1 := tsl_rec1_app None E A in
-    tLambda na A0 (tLambda (tsl_name tsl_ident na)
-                           (subst_app (lift0 1 A1) [tRel 0])
-                           (tsl_rec1_app (option_map (lift 2 2) app) E t))
-  | t => let t1 :=
+  | tRel n => ret (proj b (tRel n))
+  | tSort s => if b then ret (tSort s)
+              else ret (tLambda (nNamed "A") (tSort s) (tProd nAnon (tRel 0) (tSort s)))
+  | tCast t c A => if b then
+                    t1 <- tsl_rec fuel Σ E Γ true t ;;
+                    A1 <- tsl_rec fuel Σ E Γ true A ;;
+                    ret (tCast t1 c A1)
+                  else
+                    t1 <- tsl_rec fuel Σ E Γ true t ;;
+                    t2 <- tsl_rec fuel Σ E Γ false t ;;
+                    A2 <- tsl_rec fuel Σ E Γ false A ;;
+                    ret (tCast t2 c (tApp A2 [t1]))
+  | tProd n A B => if b then
+                    A' <- tsl_ty_param fuel Σ E Γ A ;;
+                    B1 <- tsl_rec fuel Σ E (Γ ,, vass n A) true B ;;
+                    ret (tProd n A' B1)
+                  else
+                    A' <- tsl_ty_param fuel Σ E Γ A ;;
+                    B1 <- tsl_rec fuel Σ E (Γ ,, vass n A) true B ;;
+                    B2 <- tsl_rec fuel Σ E (Γ ,, vass n A) false B ;;
+                    ret (tLambda (nNamed "f") (tProd n A' B1)
+                                 (tProd n (lift 1 0 A')
+                                        (tApp (lift 1 1 B2)
+                                              [tApp (tRel 1) [tRel 0]])))
+  | tLambda n A t => A' <- tsl_ty_param fuel Σ E Γ A ;;
+                    t' <- tsl_rec fuel Σ E (Γ ,, vass n A) b t ;;
+                    ret (tLambda n A' t')
+  | tLetIn n t A u => t' <- tsl_term fuel Σ E Γ t ;;
+                     A' <- tsl_ty_param fuel Σ E Γ A ;;
+                     u' <- tsl_rec fuel Σ E (Γ ,, vdef n t A) b u ;;
+                     ret (tLetIn n t' A' u')
+  | tApp t u => t' <- tsl_rec fuel Σ E Γ b t ;;
+               u' <- monad_map (tsl_term fuel Σ E Γ) u ;;
+               ret (tApp t' u')
+  | tConst _ _ as t
+  | tInd _ _ as t
+  | tConstruct _ _ _ as t => t' <- tsl_term fuel Σ E Γ t ;;
+                            ret (proj b t')
+  | _ => raise TranslationNotHandeled
+  end
+  end
+with tsl_term  (fuel : nat) (Σ : global_context) (E : tsl_table) (Γ : context) (t : term) {struct fuel}
+  : tsl_result term :=
+  match fuel with
+  | O => raise NotEnoughFuel
+  | S fuel =>
   match t with
-  | tRel k => tRel (2 * k)
-  | tSort s => tLambda (nNamed "A") (tSort s) (tProd nAnon (tRel 0) (tSort s))
-
-  | tProd na A B =>
-    let A0 := tsl_rec0 0 A in
-    let A1 := tsl_rec1 E A in
-    let B0 := tsl_rec0 1 B in
-    let B1 := tsl_rec1 E B in
-    let ΠAB0 := tProd na A0 B0 in
-    tLambda (nNamed "f") ΠAB0
-      (tProd na (lift0 1 A0)
-             (tProd (tsl_name tsl_ident na)
-                    (subst_app (lift0 2 A1) [tRel 0])
-                    (subst_app (lift 1 2 B1)
-                               [tApp (tRel 2) [tRel 1]])))
-  | tApp t us =>
-    let us' := concat (map (fun v => [tsl_rec0 0 v; tsl_rec1 E v]) us) in
-    mkApps (tsl_rec1 E t) us'
-
-  | tLetIn na t A u =>
-    let t0 := tsl_rec0 0 t in
-    let t1 := tsl_rec1 E t in
-    let A0 := tsl_rec0 0 A in
-    let A1 := tsl_rec1 E A in
-    let u0 := tsl_rec0 0 u in
-    let u1 := tsl_rec1 E u in
-    tLetIn na t0 A0 (tLetIn (tsl_name tsl_ident na) (lift0 1 t1)
-                            (subst_app (lift0 1 A1) [tRel 0]) u1)
-
-  | tCast t c A => let t0 := tsl_rec0 0 t in
-                  let t1 := tsl_rec1 E t in
-                  let A0 := tsl_rec0 0 A in
-                  let A1 := tsl_rec1 E A in
-                  tCast t1 c (mkApps A1 [tCast t0 c A0]) (* apply_subst ? *)
-
+  | tRel n => ret (tRel n)
+  | tCast t c A => t' <- tsl_term fuel Σ E Γ t ;;
+                  A' <- tsl_ty_param fuel Σ E Γ A ;;
+                  ret (tCast t' c A')
   | tConst s univs =>
     match lookup_tsl_table E (ConstRef s) with
-    | Some t => t
-    | None => debug "tConst" s
+    | Some t => ret t
+    | None => raise (TranslationNotFound s)
     end
   | tInd i univs =>
     match lookup_tsl_table E (IndRef i) with
-    | Some t => t
-    | None => debug "tInd" (match i with mkInd s _ => s end)
+    | Some t => ret t
+    | None => raise (TranslationNotFound (string_of_gref (IndRef i)))
     end
   | tConstruct i n univs =>
     match lookup_tsl_table E (ConstructRef i n) with
-    | Some t => t
-    | None => debug "tConstruct" (match i with mkInd s _ => s end)
+    | Some t => ret t
+    | None => raise (TranslationNotFound (string_of_gref (ConstructRef i n)))
     end
-  | tCase ik t u brs as case =>
-    let brs' := List.map (on_snd (lift0 1)) brs in
-    let case1 := tCase ik (lift0 1 t) (tRel 0) brs' in
-    match lookup_tsl_table E (IndRef (fst ik)) with
-    | Some (tInd i _univ) =>
-      tCase (i, (snd ik) * 2)
-            (tsl_rec1_app (Some (tsl_rec0 0 case1)) E t)
-            (tsl_rec1 E u)
-            (map (on_snd (tsl_rec1 E)) brs)
-    | _ => debug "tCase" (match (fst ik) with mkInd s _ => s end)
-    end
-  | _ => todo
-  end in
-  match app with Some t' => mkApp t1 (t' {3 := tRel 1} {2 := tRel 0})
-               | None => t1 end
-  end.
-Definition tsl_rec1 := tsl_rec1_app None.
+  | t => match infer Σ Γ t with
+         | Checked typ => let typ := refresh_universes typ in
+                          t1 <- tsl_rec fuel Σ E Γ true t ;;
+                        t2 <- tsl_rec fuel Σ E Γ false t ;;
+                        typ1 <- tsl_rec fuel Σ E Γ true typ ;;
+                        typ2 <- tsl_rec fuel Σ E Γ false typ ;;
+                        ret (pair typ1 typ2 t1 t2)
+        | TypeError t => raise (TypingError t)
+        end
+  end
+  end
+where "'tsl_ty_param'" := (fun fuel Σ E Γ t =>
+                        t1 <- tsl_rec fuel Σ E Γ true t ;;
+                        t2 <- tsl_rec fuel Σ E Γ false t ;;
+                        ret (pack t1 t2)).
 
-Definition tsl_mind_decl (E : tsl_table)
-           (kn kn' : kername) (mind : minductive_decl) : tsl_table * list minductive_decl.
-  refine (_, [{| ind_npars := 2 * mind.(ind_npars);
-                 ind_bodies := _;
-                 ind_universes := mind.(ind_universes)|}]).  (* FIXME always ok? *)
-  - refine (fold_left_i (fun E i ind => _ :: _ ++ E)%list mind.(ind_bodies) []).
-    + (* ind *)
-      exact (IndRef (mkInd kn i), tInd (mkInd kn' i) []).
-    + (* ctors *)
-      refine (fold_left_i (fun E k _ => _ :: E) ind.(ind_ctors) []).
-      exact (ConstructRef (mkInd kn i) k, tConstruct (mkInd kn' i) k []).
-  - refine (map_i _ mind.(ind_bodies)).
-    intros i ind.
-    refine {| ind_name := tsl_ident ind.(ind_name);
-              ind_type := _;
-              ind_kelim := ind.(ind_kelim);
-              ind_ctors := _;
-              ind_projs := [] |}. (* todo *)
-    + (* arity  *)
-      refine (let ar := subst_app (tsl_rec1 E ind.(ind_type))
-                                  [tInd (mkInd kn i) []] in
-              ar).
-    + (* constructors *)
-      refine (map_i _ ind.(ind_ctors)).
-      intros k ((name, typ), nargs).
-      refine (tsl_ident name, _, 2 * nargs).
-      refine (subst_app _ [tConstruct (mkInd kn i) k []]).
-      refine (fold_left_i (fun t0 i u  => t0 {S i := u}) _ (tsl_rec1 E typ)).
-      (* [I_n-1; ... I_0] *)
-      refine (rev (map_i (fun i _ => tInd (mkInd kn i) [])
-                              mind.(ind_bodies))).
+
+
+Instance tsl_param : Translation
+  := {| tsl_id := tsl_ident ;
+        tsl_tm := fun ΣE => tsl_term fuel (fst ΣE) (snd ΣE) [] ;
+        tsl_ty := fun ΣE => tsl_ty_param fuel (fst ΣE) (snd ΣE) [] ;
+        tsl_ind := todo |}.
+
+
+Definition TslParam := @tTranslate tsl_param.
+Definition ImplParam := @tImplement tsl_param.
+
+
+Notation "'TYPE'" := (exists A, A -> Type).
+Notation "'El' A" := (sigma (π1 A) (π2 A)) (at level 20).
+
+Definition Ty := Type.
+Set Printing Universes.
+Run TemplateProgram (TslParam emptyTC "Ty").
+Check Tyᵗ : El Tyᵗ.
+
+
+Definition mkTYPE (A₀ : Type) (Aᴿ : A₀ -> Type) : El Tyᵗ :=
+  @mk_sig Type (fun A₀ => A₀ -> Type) A₀ Aᴿ.
+
+Definition Prodᶠ (A : El Tyᵗ) (B : El A -> El Tyᵗ) : El Tyᵗ :=
+  mkTYPE
+    (forall x : El A, (B x).1)
+    (fun f₀ => forall x : El A, (B x).2 (f₀ x)).
+
+Notation "A →ᶠ B" := (Prodᶠ A (fun _ => B)) (at level 99, right associativity, B at level 200).
+Notation "'Πᶠ'  x .. y , P" := (Prodᶠ _ (fun x => .. (Prodᶠ _ (fun y => P)) ..))
+  (at level 200, x binder, y binder, right associativity).
+
+Definition Lamᶠ {A : El Tyᵗ} {B : El A -> El Tyᵗ} (f : forall x : El A, El (B x)) : El (Prodᶠ A B).
+Proof.
+unshelve refine (_ ; _).
++ refine (fun x => (f x).1).
++ refine (fun x => (f x).2).
 Defined.
 
+Notation "'λᶠ'  x .. y , t" := (Lamᶠ (fun x => .. (Lamᶠ (fun y => t)) ..))
+  (at level 200, x binder, y binder, right associativity).
 
-Run TemplateProgram (tm <- tmQuote (forall A, A -> A) ;;
-                     let tm' := tsl_rec1 [] tm in
-                     tmUnquote tm' >>= tmPrint).
-
-Run TemplateProgram (tm <- tmQuote (fun A (x : A) => x) ;;
-                     let tm' := tsl_rec1 [] tm in
-                     tmUnquote tm' >>= tmPrint).
-
-Goal ((fun f : forall A : Type, A -> A =>
-    forall (A : Type) (A0 : A -> Type) (H : A), A0 H -> A0 (f A H)) (fun A (x : A) => x)
-       = (forall (A : Type) (A0 : A -> Type) (x : A), A0 x -> A0 x)).
-reflexivity.
+Definition Appᶠ {A B} (f : El (Prodᶠ A B)) (x : El A) : El (B x).
+Proof.
+unshelve refine (_ ; _).
++ refine (f.1 x).
++ refine (f.2 x).
 Defined.
 
-
-Instance param : Translation :=
-  {| tsl_id := tsl_ident ;
-     tsl_tm := fun ΣE t => ret (tsl_rec1 (snd ΣE) t) ;
-     tsl_ty := fun '(Σ, E) t => todo "not meaningful here" ;
-     tsl_ind := fun ΣE kn kn' mind => ret (tsl_mind_decl (snd ΣE) kn kn' mind) |}.
+Notation "t · u" := (Appᶠ t u) (at level 65, left associativity).
 
 
-Definition T := forall A, A -> A.
-Run TemplateProgram (tTranslate emptyTC "T").
+Definition sigmaᵀ (A : El Tyᵗ) (P : El (A →ᶠ Tyᵗ)) : Type :=
+  sigma (El A) (fun x => El (P · x)).
+
+Definition existᵀ (A : El Tyᵗ) (P : El (A →ᶠ Tyᵗ))
+           (x : El A) (y : El (P · x)) : sigmaᵀ A P
+  := mk_sig x y.
+
+Inductive sigmaᴿ (A : El Tyᵗ) (P : El (A →ᶠ Tyᵗ)) : sigmaᵀ A P -> Type :=
+| existᴿ : forall (x : El A) (y : El (P · x)), sigmaᴿ A P (existᵀ A P x y).
+
+Definition sigmaᶠ : El (Πᶠ (A : El Tyᵗ) (P : El (A →ᶠ Tyᵗ)), Tyᵗ).
+Proof.
+refine (λᶠ A P, _).
+unshelve refine (mkTYPE _ (sigmaᴿ A P)).
+Defined.
+
+Definition existᶠ : El (Πᶠ (A : El Tyᵗ) (P : El (A →ᶠ Tyᵗ)) (x : El A) (y : El (P · x)),
+  sigmaᶠ · A · P).
+Proof.
+refine (λᶠ A P x y, _).
+refine (mk_sig (existᵀ A P x y) (existᴿ A P x y)).
+Defined.
+
+Inductive eq@{i} {A : Type@{i}} (x : A) : A -> Type@{i} :=  eq_refl : eq x x.
+
+Inductive eq2 (A : El Tyᵗ) (x : El A) :
+  forall (y : El A), eq (π1 x) (π1 y) -> Prop :=
+| refl2 : eq2 A x x (eq_refl _).
 
 
-Definition tm := ((fun A (x:A) => x) (Type -> Type) (fun x => x)).
-Run TemplateProgram (tTranslate emptyTC "tm").
+Definition eqᶠ : El (Πᶠ (A : El Tyᵗ), A →ᶠ A →ᶠ Tyᵗ).
+Proof.
+refine (λᶠ A x y, _).
+unshelve refine (mkTYPE _ _).
++ refine (eq x.1 y.1).
++ refine (eq2 A x y).
+Defined.
 
-Run TemplateProgram (TC <- tTranslate emptyTC "nat" ;;
-                     tmDefinition "nat_TC" TC ).
+Definition reflᶠ : El (Πᶠ (A : El Tyᵗ) (x : El A), eqᶠ · A · x · x).
+Proof.
+refine (λᶠ A x, _).
+unshelve refine (_; refl2 A x).
+Defined.
 
-Run TemplateProgram (tTranslate nat_TC "pred").
+Definition Falseᶠ : El Tyᵗ.
+  exists False. exact (fun _ => False).
+Defined.
+  
 
-
-Module Id1.
-  Definition ID := forall A, A -> A.
-
-  Run TemplateProgram (tTranslate emptyTC "ID").
-
-  Lemma param_ID_identity (f : ID)
-    : IDᵗ f -> forall A x, f A x = x.
-  Proof.
-    compute. intros H A x.
-    exact (H A (fun y => y = x) x (eq_refl x)).
-  Qed.
-
-  Definition toto := fun n : nat => (fun y => 0) (fun _ : Type =>  n).
-  Run TemplateProgram (tTranslate nat_TC "toto").
-
-
-  Definition my_id : ID :=
-    let n := 12 in (fun (_ : nat) y => y) 4 (fun A x => (fun _ : nat => x) n).
-
-  Run TemplateProgram (tTranslate nat_TC "my_id").
-
-
-  Definition free_thm_my_id : forall A x, my_id A x = x
-    := param_ID_identity my_id my_idᵗ.
-End Id1.
+Quote Recursively Definition sigma_prog := @sigma.
+Quote Recursively Definition eq_prog := @eq.
+Quote Recursively Definition false_prog := @False.
+Definition sigma_decl := Eval compute in
+      extract_mind_decl_from_program "Translations.sigma.sigma" sigma_prog.
+Definition eq_decl := Eval compute in
+      extract_mind_decl_from_program "Translations.tsl_param.eq" eq_prog.
+Definition false_decl := Eval compute in
+      extract_mind_decl_from_program "Coq.Init.Logic.False" false_prog.
 
 
-Module Id2.
-  Definition ID := forall A x y (p : x = y :> A), x = y.
+Definition ΣE : option tsl_context :=
+  sd <- sigma_decl ;;
+  ed <- eq_decl ;;
+  fd <- false_decl ;;
+  let Σ' := add_global_decl (InductiveDecl "Coq.Init.Logic.False" fd) (
+            add_global_decl (InductiveDecl "Translations.tsl_param.eq" ed) (
+            add_global_decl (InductiveDecl "Translations.sigma.sigma" sd)
+            ([], init_graph))) in
+  let E' := [(IndRef (mkInd "Translations.sigma.sigma" 0),
+              tConst "sigmaᶠ" []);
+             (ConstructRef (mkInd "Translations.sigma.sigma" 0) 0,
+              tConst "existᶠ" []);
+             (IndRef (mkInd "Translations.tsl_param.eq" 0), tConst "eqᶠ" []);
+             (IndRef (mkInd "Coq.Init.Logic.False" 0), tConst "Falseᶠ" [])
+            ] in
+  ret (Σ', E').
 
-  Run TemplateProgram (TC <- tTranslate emptyTC "eq" ;;
-                       TC <- tTranslate TC "ID" ;;
-                       tmDefinition "TC" TC).
-
-
-  Lemma param_ID_identity (f : ID)
-    : IDᵗ f -> forall A x y p, f A x y p = p.
-  Proof.
-    compute. intros H A x y p.
-    destruct p.
-    specialize (H A (fun y => x = y) x eq_refl x eq_refl eq_refl
-                  (eq_reflᵗ _ _ _ _)).
-    destruct H. reflexivity.
-  Qed.
-
-  Definition myf : ID
-    := fun A x y p => eq_trans (eq_trans p (eq_sym p)) p.
-
-  Run TemplateProgram (TC <- tTranslate TC "eq_sym" ;;
-                       TC <- tTranslate TC "eq_trans" ;;
-                       tTranslate TC "myf").
-
-  Definition free_thm_myf : forall A x y p, myf A x y p = p
-    := param_ID_identity myf myfᵗ.
-End Id2.
+Definition HasTwoElFstComponentᵗ : El (Tyᵗ →ᶠ Tyᵗ)
+  := λᶠ (T : El Tyᵗ), mkTYPE (exists (x y : T.1), x = y -> False) (fun _ => unit).
 
 
+Definition equiv (A B : Type) :=
+  (* Type. *)
+  exists (f : A -> B) (g : B -> A),
+    (forall x, eq (g (f x)) x) × (forall x, eq (f (g x)) x).
+
+Definition FALSE := forall X, X.
+Run TemplateProgram (TslParam emptyTC "FALSE").
+
+Proposition consistency_preservation : El FALSEᵗ -> FALSE.
+  compute.
+  intros [f _] X.
+  exact (f (X; fun _ => unit)).
+Defined.
+
+Quote Definition equiv_ := Eval compute in equiv.
 
 
+Check "go".
 
-Module Vectors.
-  Import Vector.
-  Run TemplateProgram (tTranslate nat_TC "t").
-End Vectors.
+Run TemplateProgram (match ΣE with
+                     | None => tmFail "bug: no tsl_ctx"
+                     | Some ΣE =>
+                       ΣE <- TslParam ΣE "equiv" ;;
+                       (* tmPrint ΣE' ;; *)
+                       tmPrint "lo" ;;
+                       H <- ImplParam ΣE "notUnivalence"
+                       (exists A B : Type, (equiv A B) × exists P, P A × ((P B) -> False)) ;;
+                       (* (exists A : Type, (equiv A A)) ;; *)
+                       tmPrint "done"
+                     end).
+Check "proof".
+Next Obligation.
+simple refine (existᶠ · _ · _ · _ · _).
+exact (bool:Type; fun _=> unit:Type).
+simple refine (existᶠ · _ · _ · _ · _).
+exact (unit:Type; fun _ => bool:Type).
+simple refine (existᶠ · _ · _ · _ · _).
+- simple refine (existᶠ · _ · _ · _ · _).
+  exists π2. exact π1.
+  simple refine (existᶠ · _ · _ · _ · _).
+  exists π2. exact π1.
+  simple refine (existᶠ · _ · _ · _ · _);
+    cbn; unshelve econstructor; reflexivity.
+- simple refine (existᶠ · _ · _ · _ · _).
+  exact HasTwoElFstComponentᵗ.
+  simple refine (existᶠ · _ · _ · _ · _).
+  + cbn. refine (_; tt). exists true. exists false.
+    discriminate 1.
+  + compute.
+    split; (intro p;
+            destruct p as [p _];
+            destruct p as [[] [[] p]];
+            contradiction p; reflexivity).
+Defined.
 
-Require Import Even.
-Run TemplateProgram (tTranslate nat_TC "even").
-
-Definition rev_type := forall A, list A -> list A.
-Run TemplateProgram (TC <- tTranslate emptyTC "list" ;;
-                     TC <- tTranslate TC "rev_type" ;;
-                     tmDefinition "list_TC" TC ).
-
-
-
-(* Definition isequiv (A B : Type) (f : A -> B) := *)
-(*   exists (g : B -> A), (forall x, g (f x) = x) × (forall y, f (g y) = y). *)
-
-(* Definition equiv_id A : isequiv A A (fun x => x). *)
-(*   unshelve econstructor. exact (fun y => y). *)
-(*   split; reflexivity. *)
-(* Defined. *)
-
-(* Run TemplateProgram (TC <- tTranslate [] "sigma" ;; *)
-(*                      TC <- tTranslate TC "eq" ;; *)
-(*                      TC <- tTranslate TC "isequiv" ;; *)
-(*                      TC <- tTranslate TC "equiv_id" ;; *)
-(*                      tmDefinition "TC" TC). *)
-
-(* Quote Definition eq_rect_Type_ := (forall (A : Type) (x : A) (P : A -> Type), *)
-(* P x -> forall y : A, x = y -> P y). *)
-(* Make Definition eq_rect_Typeᵗ :=  ltac:(let t:= eval compute in (tsl_rec1 TC eq_rect_Type_) in exact t). *)
-
-(* Lemma eq_rectᵗ : eq_rect_Typeᵗ eq_rect. *)
-(*   compute. intros A Aᵗ x xᵗ P Pᵗ X X0 y yᵗ H H0.  *)
-(*     by destruct H0. *)
-(* Defined. *)
-
-(* Definition TC' := (ConstRef "Coq.Init.Logic.eq_rect", tConst "eq_rectᵗ" []) :: TC. *)
-
-(* Definition eq_to_iso A B : A = B -> exists f, isequiv A B f. *)
-(*   refine (eq_rect _ (fun B => exists f : A -> B, isequiv A B f) _ _). *)
-(*   econstructor. *)
-(*   eapply equiv_id. *)
-(* Defined. *)
-
-(* Definition UA := forall A B, isequiv _ _ (eq_to_iso A B). *)
-
-(* Run TemplateProgram (TC <- tTranslate TC' "eq_to_iso" ;; *)
-(*                      tTranslate TC "UA"). *)
-
-(* Arguments isequiv {A B} _. *)
-(* Arguments isequivᵗ {_ _ _ _} _ _. *)
-(* Arguments eqᵗ {A Aᵗ x xᵗ H} _ _.  *)
-
-(* Axiom ua : UA. *)
-
-(* Goal UAᵗ ua. *)
-(*   intros A Aᵗ B Bᵗ.  *)
-(*   unshelve econstructor. *)
-(*   - intros [f e] []. clear f e. *)
-(*     assert (forall H, isequiv (π1ᵗ H)). { *)
-(*       destruct π2ᵗ. destruct π2ᵗ. *)
-(*       intro x. unshelve econstructor. *)
-(*       by refine (fun y => eq_rect _ Aᵗ (π1ᵗ0 _ y) _ _). *)
-(*       split. { intro. *)
+Check "ok!".
